src/tree_of_strategy.lean
@@ -4,116 +4,100 @@ open encodable denumerable
 
 attribute [simp] set.set_of_app_iff
 
-universes u v
+structure strategy (α : Type*) :=
+(omega_ordering : omega_ordering (Tree 1 × ℕ))
+(computation_init : α)
+(computation : option (Tree 1 × ℕ) → α → (infinity ⊕ zero) × α)
 
-structure strategy (α : Type u) [decidable_eq α] :=
-(par₀ : Tree α 0 → ℕ)
-(par₁ : Tree α 1 → ℕ)
-(computation : Tree α 0 → option (Tree α 1 × ℕ) → infinity ⊕ Tree' α 0)
-(omega_ordering : omega_ordering (Tree α 1 × ℕ))
-#check strategy
 namespace strategy
-variables {α : Type*} [decidable_eq α]
-variables (S : strategy α)
+variables {α : Type*} (S : strategy α)
 
 namespace approx
 
-def up_inv (η : Tree α 1) {μ : Tree α 0} (υ : branch μ → option (Tree α 1)) : list (branch μ) :=
+def derivative (η : Tree 1) {μ : Tree 0} (υ : branch μ → option (Tree 1)) : list (branch μ) :=
 μ.branches.filter (λ a, υ a = η)
 
-lemma up_inv_ordered (η : Tree α 1) {μ : Tree α 0} (υ : branch μ → option (Tree α 1)) :
-  (up_inv η υ).ordered (<) :=
-by { simp[up_inv], exact list.ordered_filter _ (branch.branches_ordered μ) }
+lemma derivative_ordered (η : Tree 1) {μ : Tree 0} (υ : branch μ → option (Tree 1)) :
+  (derivative η υ).ordered (<) :=
+by { simp[derivative], exact list.ordered_filter _ (branch.branches_ordered μ) }
 
-lemma up_inv_cons (η : Tree α 1) {μ : Tree α 0} {x} (υ : branch (x :: μ) → option (Tree α 1)) :
-  (up_inv η υ).map subtype.val =
-  if υ ⟨μ, by simp⟩ = ↑η
-    then μ :: (@up_inv _ _ η μ (λ ν, υ ν.cons')).map subtype.val
-    else (@up_inv _ _ η μ (λ ν, υ ν.cons')).map subtype.val :=
-begin
-  simp[up_inv, list.filter],
-  by_cases C : υ ⟨μ, by simp⟩ = ↑η; simp[C],
-  { simp[list.map_filter, function.comp], unfold_coes },
-  { simp[list.map_filter, function.comp], unfold_coes }
-end
-
-lemma up_inv_suffx (η : Tree α 1) {μ₁ μ₂ : Tree α 0} (s : μ₁ ⊆ μ₂)
-  (υ₁ : branch μ₁ → option (Tree α 1)) (υ₂ : branch μ₂ → option (Tree α 1))
+lemma derivative_suffx (η : Tree 1) {μ₁ μ₂ : Tree 0} (s : μ₁ ⊆ μ₂)
+  (υ₁ : branch μ₁ → option (Tree 1)) (υ₂ : branch μ₂ → option (Tree 1))
   (con : ∀ ν₁ : branch μ₁, υ₁ ν₁ = υ₂ (ν₁.extend s)) :
-  (up_inv η υ₁).map (branch.extend s) <:+ up_inv η υ₂ :=
+  (derivative η υ₁).map (branch.extend s) <:+ derivative η υ₂ :=
 begin
-  simp[up_inv],
+  simp[derivative],
   have : (μ₁.branches.filter (λ a, υ₁ a = ↑η)).map (branch.extend s) =
     (((μ₁.branches).map (branch.extend s)).filter (λ a, υ₂ a = ↑η)),
   { simp[list.map_filter, function.comp, con], unfold_coes, congr },
   rw this, exact (list.is_suffix.filter _ (branch.branches_suffix_of_suffix s))
 end
 
-@[simp] lemma up_inv_mem_iff {η : Tree α 1} {μ : Tree α 0} {υ : branch μ → option (Tree α 1)} {μ₀ : branch μ} :
-  μ₀ ∈ up_inv η υ ↔ υ μ₀ = η :=
-by simp[up_inv]
+@[simp] lemma derivative_mem_iff {η : Tree 1} {μ : Tree 0} {υ : branch μ → option (Tree 1)} {μ₀ : branch μ} :
+  μ₀ ∈ derivative η υ ↔ υ μ₀ = η :=
+by simp[derivative]
 
-def weight (η : Tree α 1) {μ : Tree α 0} (υ : branch μ → option (Tree α 1)) : ℕ := (up_inv η υ).length
+def weight (η : Tree 1) {μ : Tree 0} (υ : branch μ → option (Tree 1)) : ℕ := (derivative η υ).length
 
-lemma of_pos_weight {η : Tree α 1} {μ : Tree α 0} (υ : branch μ → option (Tree α 1)) (pos : 0 < weight η υ) :
+lemma of_pos_weight {η : Tree 1} {μ : Tree 0} (υ : branch μ → option (Tree 1)) (pos : 0 < weight η υ) :
   ∃ μ₀ : branch μ, υ μ₀ = η :=
-⟨_, up_inv_mem_iff.mp (list.nth_le_mem _ _ pos)⟩
+⟨_, derivative_mem_iff.mp (list.nth_le_mem _ _ pos)⟩
 
-lemma pos_weight_of {η : Tree α 1} {μ : Tree α 0} (υ : branch μ → option (Tree α 1))
+lemma pos_weight_of {η : Tree 1} {μ : Tree 0} (υ : branch μ → option (Tree 1))
   (h : ∃ μ₀ : branch μ, υ μ₀ = η) : 0 < weight η υ :=
 by { rcases h with ⟨μ₀, h⟩, 
-     exact list.length_pos_of_mem ((@up_inv_mem_iff _ _ η μ υ μ₀).mpr h) }
+     exact list.length_pos_of_mem ((@derivative_mem_iff η μ υ μ₀).mpr h) }
 
-lemma le_weight_of_suffix (η : Tree α 1) {μ₁ μ₂ : Tree α 0} (ss : μ₁ <:+ μ₂)
-  (υ₁ : branch μ₁ → option (Tree α 1)) (υ₂ : branch μ₂ → option (Tree α 1))
+lemma le_weight_of_suffix (η : Tree 1) {μ₁ μ₂ : Tree 0} (ss : μ₁ <:+ μ₂)
+  (υ₁ : branch μ₁ → option (Tree 1)) (υ₂ : branch μ₂ → option (Tree 1))
   (con : ∀ ν₁ : branch μ₁, υ₁ ν₁ = υ₂ (ν₁.extend ss)) :
   weight η υ₁ ≤ weight η υ₂ :=
-by { have := list.length_le_of_infix (list.infix_of_suffix (up_inv_suffx η ss υ₁ υ₂ con)),
+by { have := list.length_le_of_infix (list.infix_of_suffix (derivative_suffx η ss υ₁ υ₂ con)),
      simp at this, exact this }
 
-def get_up_inv (η : Tree α 1) {μ : Tree α 0} (υ : branch μ → option (Tree α 1)) : option (branch μ) :=
-(up_inv η υ).get_elem_r (λ μ₀, out μ₀ = ∞)
+def convergent_derivative (η : Tree 1) {μ : Tree 0} (υ : branch μ → option (Tree 1)) : option (branch μ) :=
+(derivative η υ).get_elem_r (λ μ₀, out μ₀ = ∞)
 
-lemma is_some_of_out_infinity {η : Tree α 1} {μ : Tree α 0} (υ : branch μ → option (Tree α 1)) (μ₀ : branch μ)
-  (infty : out μ₀ = ∞) (up : υ μ₀ = η) : (get_up_inv η υ).is_some :=
-by { cases C : get_up_inv η υ; simp[get_up_inv, list.get_elem_r_eq_none_iff_mem] at C ⊢,
+lemma is_some_of_out_infinity {η : Tree 1} {μ : Tree 0} (υ : branch μ → option (Tree 1)) (μ₀ : branch μ)
+  (infty : out μ₀ = ∞) (up : υ μ₀ = η) : (convergent_derivative η υ).is_some :=
+by { cases C : convergent_derivative η υ; simp[convergent_derivative, list.get_elem_r_eq_none_iff_mem] at C ⊢,
      exfalso, exact C _ up infty }
 
-lemma get_up_inv_eq_some_iff
-  {η : Tree α 1} {μ : Tree α 0} {υ : branch μ → option (Tree α 1)} {μ₀ : branch μ} :
-  get_up_inv η υ = ↑μ₀ ↔ (out μ₀ = ∞) ∧ (υ μ₀ = η) ∧ (∀ μ₁, μ₁ < μ₀ → υ μ₁ = η → out μ₁ ≠ ∞) :=
+lemma convergent_derivative_eq_some_iff
+  {η : Tree 1} {μ : Tree 0} {υ : branch μ → option (Tree 1)} {μ₀ : branch μ} :
+  convergent_derivative η υ = ↑μ₀ ↔ (out μ₀ = ∞) ∧ (υ μ₀ = η) ∧ (∀ μ₁, μ₁ < μ₀ → υ μ₁ = η → out μ₁ ≠ ∞) :=
 begin
-  simp[get_up_inv, list.get_elem_r_eq_some_iff], split,
+  simp[convergent_derivative, list.get_elem_r_eq_some_iff], split,
   { rintros ⟨n, eqn_μ₀, infty₀, min⟩,
-    have up₀ : μ₀ ∈ up_inv η υ, from list.mem_iff_rnth.mpr ⟨_, eqn_μ₀⟩, simp at up₀,
+    have up₀ : μ₀ ∈ derivative η υ, from list.mem_iff_rnth.mpr ⟨_, eqn_μ₀⟩, simp at up₀,
     refine ⟨infty₀, up₀, λ μ₁ lt up₁, _⟩,
-    have : ∃ n₁, (up_inv η υ).rnth n₁ = ↑μ₁, from list.mem_iff_rnth.mp (up_inv_mem_iff.mpr up₁),
+    have : ∃ n₁, (derivative η υ).rnth n₁ = ↑μ₁, from list.mem_iff_rnth.mp (derivative_mem_iff.mpr up₁),
     rcases this with ⟨m, eqn_μ₁⟩,
-    have lt : m < n, from (list.ordered_isomorphism (up_inv_ordered η υ) eqn_μ₁ eqn_μ₀).mpr lt,
+    have lt : m < n, from (list.ordered_isomorphism (derivative_ordered η υ) eqn_μ₁ eqn_μ₀).mpr lt,
     exact min _ _ lt eqn_μ₁ },
   { rintros ⟨infty₀, up₀, min⟩, 
-    have : ∃ n, (up_inv η υ).rnth n = ↑μ₀,
-    { have : μ₀ ∈ up_inv η υ, { simp[up₀] }, exact list.mem_iff_rnth.mp this },
+    have : ∃ n, (derivative η υ).rnth n = ↑μ₀,
+    { have : μ₀ ∈ derivative η υ, { simp[up₀] }, exact list.mem_iff_rnth.mp this },
     rcases this with ⟨n, eqn_μ₀⟩,
     refine ⟨n, eqn_μ₀, infty₀, λ m μ₁ eqn_m eqn_μ₁ infty₁, _⟩,
-    have lt : μ₁ < μ₀, from list.ordered_mono (up_inv_ordered η υ) eqn_m eqn_μ₁ eqn_μ₀,
-    have up : μ₁ ∈ up_inv η υ, from list.mem_iff_rnth.mpr ⟨_, eqn_μ₁⟩, simp at up,
+    have lt : μ₁ < μ₀, from list.ordered_mono (derivative_ordered η υ) eqn_m eqn_μ₁ eqn_μ₀,
+    have up : μ₁ ∈ derivative η υ, from list.mem_iff_rnth.mpr ⟨_, eqn_μ₁⟩, simp at up,
     exact min _ lt up infty₁ }
 end
 
-lemma get_up_inv_eq_none_iff {η : Tree α 1} {μ : Tree α 0} {υ : branch μ → option (Tree α 1)} :
-  get_up_inv η υ = none ↔ (∀ μ₀ : branch μ, υ μ₀ = η → out μ₀ ≠ ∞) :=
-by simp[get_up_inv, list.get_elem_r_eq_none_iff_mem]
+lemma convergent_derivative_eq_none_iff {η : Tree 1} {μ : Tree 0} {υ : branch μ → option (Tree 1)} :
+  convergent_derivative η υ = none ↔ (∀ μ₀ : branch μ, υ μ₀ = η → out μ₀ ≠ ∞) :=
+by simp[convergent_derivative, list.get_elem_r_eq_none_iff_mem]
 
-lemma get_up_inv_of_suffx (η : Tree α 1) {μ₁ μ₂ : Tree α 0} (ss : μ₁ <:+ μ₂)
-  (υ₁ : branch μ₁ → option (Tree α 1)) (υ₂ : branch μ₂ → option (Tree α 1))
+lemma convergent_derivative_of_suffx (η : Tree 1) {μ₁ μ₂ : Tree 0} (ss : μ₁ <:+ μ₂)
+  (υ₁ : branch μ₁ → option (Tree 1)) (υ₂ : branch μ₂ → option (Tree 1))
   (con : ∀ ν₁ : branch μ₁, υ₁ ν₁ = υ₂ (ν₁.extend ss)) {ν : branch μ₁}
-  (h : get_up_inv η υ₁ = some ν) :
-  get_up_inv η υ₂ = some (ν.extend ss) :=
+  (h : convergent_derivative η υ₁ = some ν) :
+  convergent_derivative η υ₂ = some (ν.extend ss) :=
 begin
-  apply get_up_inv_eq_some_iff.mpr,
+  apply convergent_derivative_eq_some_iff.mpr,
   have : out ν = ∞ ∧ υ₁ ν = ↑η ∧ ∀ (μ₁' : branch μ₁), μ₁' < ν → υ₁ μ₁' = ↑η → out μ₁' ≠ ∞,
-    from get_up_inv_eq_some_iff.mp h,
+    from convergent_derivative_eq_some_iff.mp h,
   rcases this with ⟨out_infty, eqn_up, min⟩,
   have : out ⟨↑ν, list.suffix_of_is_initial_is_initial ν.property ss⟩ = out ν,
     from suffix_out_eq rfl ss,
@@ -124,28 +108,28 @@ begin
   contradiction
 end
 
-def lambda' {μ : Tree α 0} (υ : branch μ → option (Tree α 1)) : ℕ → Tree α 1
+def lambda' {μ : Tree 0} (υ : branch μ → option (Tree 1)) : ℕ → Tree 1
 | 0       := []
 | (n + 1) :=
     if 0 < weight (lambda' n) υ then
-      if h : (get_up_inv (lambda' n) υ).is_some then
+      if h : (convergent_derivative (lambda' n) υ).is_some then
         sum.inr (option.get h).val :: lambda' n
       else ∞ :: lambda' n
     else lambda' n
 
-def lambda {μ : Tree α 0} (υ : branch μ → option (Tree α 1)) : Tree α 1 := lambda' υ μ.length
+def lambda {μ : Tree 0} (υ : branch μ → option (Tree 1)) : Tree 1 := lambda' υ μ.length
 
-lemma lambda'_length {μ : Tree α 0} (υ : branch μ → option (Tree α 1)) :
+lemma lambda'_length {μ : Tree 0} (υ : branch μ → option (Tree 1)) :
   ∀ n, (lambda' υ n).length ≤ n
 | 0       := by simp[lambda']
 | (n + 1) :=
     begin
       by_cases C₁ : 0 < weight (lambda' υ n) υ; simp[lambda', C₁],
-      { cases C₂ : get_up_inv (lambda' υ n) υ; simp[C₂]; refine lambda'_length n },
+      { cases C₂ : convergent_derivative (lambda' υ n) υ; simp[C₂]; refine lambda'_length n },
       exact le_add_right (lambda'_length n)
     end    
   
-lemma lambda'_mono {μ : Tree α 0} (υ : branch μ → option (Tree α 1)) : ∀ {n m : ℕ} (le : n ≤ m),
+lemma lambda'_mono {μ : Tree 0} (υ : branch μ → option (Tree 1)) : ∀ {n m : ℕ} (le : n ≤ m),
   lambda' υ n ⊆ lambda' υ m :=
 begin
   suffices : ∀ n m, lambda' υ n <:+ lambda' υ (n + m),
@@ -155,25 +139,25 @@ begin
   { refl },
   { simp[←nat.add_one, ←add_assoc, lambda'],
     by_cases C₁ : 0 < weight (lambda' υ (n + m)) υ; simp[C₁],
-    { cases C₂ : get_up_inv (lambda' υ (n + m)) υ; simp;
+    { cases C₂ : convergent_derivative (lambda' υ (n + m)) υ; simp;
       exact IH.trans (list.suffix_cons _ (lambda' υ (n + m))) },
     exact IH }
 end
 
-lemma lambda'_length_mono {μ : Tree α 0} (υ : branch μ → option (Tree α 1)) {n m : ℕ} (le : n ≤ m) :
+lemma lambda'_length_mono {μ : Tree 0} (υ : branch μ → option (Tree 1)) {n m : ℕ} (le : n ≤ m) :
   (lambda' υ n).length ≤ (lambda' υ m).length :=
 list.length_le_of_infix (list.infix_of_suffix (lambda'_mono υ le))
 
-lemma weight0_of_lambda'_length_lt {μ : Tree α 0} {υ : branch μ → option (Tree α 1)} : ∀ {n : ℕ}
+lemma weight0_of_lambda'_length_lt {μ : Tree 0} {υ : branch μ → option (Tree 1)} : ∀ {n : ℕ}
  (h : (lambda' υ n).length < n), weight (lambda' υ n) υ = 0
 | 0       h := by simp at h; contradiction
 | (n + 1) h := by { simp[lambda'] at h ⊢,
     by_cases C : 0 < weight (lambda' υ n) υ; simp[C] at h ⊢,
-    { exfalso, cases get_up_inv (lambda' υ n) υ; simp at h ⊢;
+    { exfalso, cases convergent_derivative (lambda' υ n) υ; simp at h ⊢;
       { simp[weight0_of_lambda'_length_lt h] at C, contradiction } },
     { simp at C, exact C } }
 
-lemma constant_of_lambda'_length_lt {μ : Tree α 0} {υ : branch μ → option (Tree α 1)} : ∀ {n m : ℕ} (le : n ≤ m)
+lemma constant_of_lambda'_length_lt {μ : Tree 0} {υ : branch μ → option (Tree 1)} : ∀ {n m : ℕ} (le : n ≤ m)
   (h : (lambda' υ n).length < n), lambda' υ m = lambda' υ n := 
 begin
   suffices : ∀ (n m : ℕ) (h : (lambda' υ n).length < n),
@@ -187,7 +171,7 @@ begin
     refine ⟨nat.lt.step IH.1, IH.2⟩ }
 end
 
-lemma length_eq_of_pos_weight {μ : Tree α 0} {υ : branch μ → option (Tree α 1)} {n}
+lemma length_eq_of_pos_weight {μ : Tree 0} {υ : branch μ → option (Tree 1)} {n}
   (h : 0 < weight (lambda' υ n) υ) : (lambda' υ n).length = n :=
 begin
   have C : (lambda' υ n).length < n ∨ (lambda' υ n).length = n, from lt_or_eq_of_le (lambda'_length υ n),
@@ -195,12 +179,12 @@ begin
   { exfalso,
     have : lambda' υ (n + 1) = lambda' υ n, from constant_of_lambda'_length_lt (by simp) C,
     simp[lambda', h] at this,
-    cases C₁ : get_up_inv (lambda' υ n) υ; simp[C₁] at this; contradiction },
+    cases C₁ : convergent_derivative (lambda' υ n) υ; simp[C₁] at this; contradiction },
     exact C
 end
 
-lemma lambda'_suffix_eq {μ : Tree α 0} (υ : branch μ → option (Tree α 1)) : ∀ {n : ℕ}
-  {x} {η : Tree α 1} (hη : x :: η <:+ lambda' υ n),
+lemma lambda'_suffix_eq {μ : Tree 0} (υ : branch μ → option (Tree 1)) : ∀ {n : ℕ}
+  {x} {η : Tree 1} (hη : x :: η <:+ lambda' υ n),
   lambda' υ η.length = η ∧ lambda' υ (η.length + 1) = x :: η
 | 0       x η h := by { exfalso, simp[lambda', *] at * }
 | (n + 1) x η h :=
@@ -208,7 +192,7 @@ lemma lambda'_suffix_eq {μ : Tree α 0} (υ : branch μ → option (Tree α 1))
       simp[lambda'] at h,
       by_cases C₁ : 0 < weight (lambda' υ n) υ; simp[C₁] at h,
       { have len : (lambda' υ n).length = n, from length_eq_of_pos_weight C₁,
-        cases C₂ : get_up_inv (lambda' υ n) υ with ν; simp[C₂] at h,
+        cases C₂ : convergent_derivative (lambda' υ n) υ with ν; simp[C₂] at h,
         { have C₃ : x :: η = ∞ :: lambda' υ n ∨ x :: η <:+ lambda' υ n, from list.suffix_cons_iff.mp h,
           cases C₃,
           { simp at C₃, have : η.length = n, { simp[C₃, len] },
@@ -223,7 +207,7 @@ lemma lambda'_suffix_eq {μ : Tree α 0} (υ : branch μ → option (Tree α 1))
       exact @lambda'_suffix_eq n x η h
     end
 
-lemma exists_up_inv {μ : Tree α 0} {υ : branch μ → option (Tree α 1)} {n : ℕ}
+lemma exists_derivative {μ : Tree 0} {υ : branch μ → option (Tree 1)} {n : ℕ}
   (η₀ : branch (lambda' υ n)) : ∃ μ₀ : branch μ, υ μ₀ = η₀ :=
 begin
   have : lambda' υ (list.length ↑η₀) = η₀ ∧ lambda' υ (list.length ↑η₀ + 1) = out η₀ :: η₀.val,
@@ -232,19 +216,19 @@ begin
   simp[lambda', lmm₁] at lmm₂,
   by_cases C : 0 < weight ↑η₀ υ; simp[C] at lmm₂,
   { simp[weight] at C,
-    have := up_inv_mem_iff.mp (list.nth_le_mem _ _ C), 
+    have := derivative_mem_iff.mp (list.nth_le_mem _ _ C), 
     refine ⟨_, this⟩ },
   { contradiction }
 end
 
-lemma branch_of_out_inr {μ : Tree α 0} (υ : branch μ → option (Tree α 1)) {n : ℕ}
-  {η : branch (lambda' υ n)} {μ₀ : Tree α 0} (h : out η = sum.inr μ₀) : μ₀ ⊂ᵢ μ :=
+lemma branch_of_out_inr {μ : Tree 0} (υ : branch μ → option (Tree 1)) {n : ℕ}
+  {η : branch (lambda' υ n)} {μ₀ : Tree 0} (h : out η = sum.inr μ₀) : μ₀ ⊂ᵢ μ :=
 begin
   have : lambda' υ (list.length ↑η) = η.val ∧ lambda' υ (list.length ↑η + 1) = sum.inr μ₀ :: η.val,
   { simp[out_eq_iff] at h, refine lambda'_suffix_eq υ h },
   rcases this with ⟨eqn_η, eqn_η'⟩, simp[lambda', eqn_η] at eqn_η',
   by_cases C₁ : 0 < weight ↑η υ; simp[C₁] at eqn_η',
-  { cases C₂ : get_up_inv ↑η υ with ν; simp[C₂] at eqn_η',
+  { cases C₂ : convergent_derivative ↑η υ with ν; simp[C₂] at eqn_η',
     { exfalso, have := list.head_eq_of_cons_eq eqn_η', simp* at * },
     { have : ν.val = μ₀,
         from sum.inr.inj (list.head_eq_of_cons_eq eqn_η'),
@@ -254,26 +238,26 @@ begin
 end
 
 theorem lambda'_convergent_out_iff
-  {μ : Tree α 0} (υ : branch μ → option (Tree α 1)) {n : ℕ} {η : branch (lambda' υ n)} {μ₀ : branch μ} :
+  {μ : Tree 0} (υ : branch μ → option (Tree 1)) {n : ℕ} {η : branch (lambda' υ n)} {μ₀ : branch μ} :
   out η = sum.inr μ₀.val ↔ (out μ₀ = ∞) ∧ (υ μ₀ = η) ∧ (∀ μ₁, μ₁ < μ₀ → υ μ₁ = η → out μ₁ ≠ ∞) :=
 begin
   have : lambda' υ (list.length ↑η) = η ∧ lambda' υ (list.length ↑η + 1) = out η :: η.val,
     from lambda'_suffix_eq υ (suffix_out_cons η),
   rcases this with ⟨eqn_η, eqn_η'⟩, simp[lambda', eqn_η] at eqn_η',
   by_cases C₁ : 0 < weight ↑η υ; simp[C₁] at eqn_η'; simp[eqn_η] at*,
-  { cases C₂ : get_up_inv ↑η υ with μ₁; simp[C₂] at eqn_η',
+  { cases C₂ : convergent_derivative η υ with μ₁; simp[C₂] at eqn_η',
     { have eqn₁ : ∞ = out η, from list.head_eq_of_cons_eq eqn_η', simp[←eqn₁], 
       intros h₁ h₂, exfalso,
-      have : ∀ μ₀, υ μ₀ = η → ¬out μ₀ = ∞ := get_up_inv_eq_none_iff.mp C₂,
+      have : ∀ μ₀, υ μ₀ = η → ¬out μ₀ = ∞ := convergent_derivative_eq_none_iff.mp C₂,
       exact this _ h₂ h₁ },
     { have eqn₁ : sum.inr μ₁.val = out η, from list.head_eq_of_cons_eq eqn_η',
-      have := @get_up_inv_eq_some_iff _ _ ↑η μ υ μ₀,
+      have := @convergent_derivative_eq_some_iff η μ υ μ₀,
       simp[←this, C₂, ←eqn₁, ←subtype.ext_iff] } },
   { contradiction }
 end
 
 theorem lambda'_divergent_out_iff
-  {μ : Tree α 0} (υ : branch μ → option (Tree α 1)) {n : ℕ} {η : branch (lambda' υ n)} :
+  {μ : Tree 0} (υ : branch μ → option (Tree 1)) {n : ℕ} {η : branch (lambda' υ n)} :
   out η = ∞ ↔ (∀ μ₀, υ μ₀ = η → out μ₀ ≠ ∞) :=
 ⟨λ h,
   begin
@@ -281,8 +265,8 @@ theorem lambda'_divergent_out_iff
       from lambda'_suffix_eq υ (suffix_out_cons η),
     rcases this with ⟨eqn_η, eqn_η'⟩, simp[lambda', eqn_η] at eqn_η',
     by_cases C₁ : 0 < weight ↑η υ; simp[lambda', C₁] at eqn_η',
-    { cases C₂ : get_up_inv ↑η υ with ν; simp[C₂] at eqn_η',
-      { exact get_up_inv_eq_none_iff.mp C₂ },
+    { cases C₂ : convergent_derivative ↑η υ with ν; simp[C₂] at eqn_η',
+      { exact convergent_derivative_eq_none_iff.mp C₂ },
       { exfalso, have := list.head_eq_of_cons_eq eqn_η', simp* at* } },
     { contradiction }
   end, λ h,
@@ -290,13 +274,13 @@ theorem lambda'_divergent_out_iff
     have : lambda' υ (list.length ↑η) = η ∧ lambda' υ (list.length ↑η + 1) = out η :: η.val,
       from lambda'_suffix_eq υ (suffix_out_cons η),
     rcases this with ⟨eqn_η, eqn_η'⟩, simp[lambda', eqn_η] at eqn_η',
-    have lmm₁ : 0 < weight η.val υ, from pos_weight_of υ (exists_up_inv η),
-    have lmm₂ : get_up_inv η.val υ = none, from get_up_inv_eq_none_iff.mpr h, simp at*,
+    have lmm₁ : 0 < weight η.val υ, from pos_weight_of υ (exists_derivative η),
+    have lmm₂ : convergent_derivative η.val υ = none, from convergent_derivative_eq_none_iff.mpr h, simp at*,
     simp[lambda', eqn_η, lmm₁, lmm₂] at eqn_η',
     exact eq.symm (list.head_eq_of_cons_eq eqn_η')
   end⟩
 
-private lemma length_le_of_surj {n m : ℕ} {μ : Tree α m} (f : branch μ → option (Tree α n)) {η : Tree α n}
+private lemma length_le_of_surj {n m : ℕ} {μ : Tree m} (f : branch μ → option (Tree n)) {η : Tree n}
   (h : ∀ η₀ : branch η, ∃ μ₀ : branch μ, f μ₀ = η₀) : η.length ≤ μ.length :=
 begin
   have eqn₁ : ((branch.branch_univ μ).image f).card ≤ μ.length,
@@ -307,12 +291,12 @@ begin
     have eqn₁ : ((branch.branch_univ' η).image some).card ≤ ((branch.branch_univ μ).image f).card,
       from finset.card_le_of_subset this,
     have eqn₂ : ((branch.branch_univ' η).image some).card = (branch.branch_univ' η).card,
-      from finset.card_image_of_injective (branch.branch_univ' η) (option.some_injective (Tree α n)),
+      from finset.card_image_of_injective (branch.branch_univ' η) (option.some_injective (Tree n)),
     simp at eqn₂, simp [eqn₂] at eqn₁, exact eqn₁ },
   exact le_trans eqn₂ eqn₁
 end
 
-lemma lambda_eq_of_le {μ : Tree α 0} (υ : branch μ → option (Tree α 1)) : ∀ {n : ℕ} (h : μ.length ≤ n),
+lemma lambda_eq_of_le {μ : Tree 0} (υ : branch μ → option (Tree 1)) : ∀ {n : ℕ} (h : μ.length ≤ n),
   lambda' υ n = lambda υ :=
 begin
   suffices :
@@ -333,7 +317,7 @@ begin
   rcases this with ⟨μ₀, eqn⟩,
   have : ∀ (η₀ : branch (∞ :: (lambda υ))), ∃ (μ₀ : branch μ), υ μ₀ = ↑η₀,
   { intros η₀,
-    have : ∀ (η₀ : branch (lambda υ)), ∃ (μ₀ : branch μ), υ μ₀ = ↑η₀, from @exists_up_inv _ _ μ υ μ.length,
+    have : ∀ (η₀ : branch (lambda υ)), ∃ (μ₀ : branch μ), υ μ₀ = ↑η₀, from @exists_derivative μ υ μ.length,
     have C₁ : η₀.val = lambda υ ∨ η₀.val ⊂ᵢ lambda υ, from list.is_initial_cons_iff.mp η₀.property,
     cases C₁,
     { exact ⟨μ₀, by simp[eqn, ←C₁]⟩ },
@@ -343,7 +327,7 @@ begin
   exact ((lambda υ).length).not_succ_le_self (le_trans this C)
 end
 
-private lemma lambda'_eq_lambda'_length {μ : Tree α 0} (υ : branch μ → option (Tree α 1)) (n : ℕ) :
+private lemma lambda'_eq_lambda'_length {μ : Tree 0} (υ : branch μ → option (Tree 1)) (n : ℕ) :
   lambda' υ n = lambda' υ (lambda' υ n).length :=
 begin
   have le : (lambda' υ n).length ≤ n, from lambda'_length υ n,
@@ -355,7 +339,7 @@ begin
   { exact eq.symm (list.eq_of_suffix_of_length_eq (lambda'_mono υ le) C) }
 end 
 
-lemma lambda_eq_of_le' {μ : Tree α 0} {υ : branch μ → option (Tree α 1)} {n : ℕ} (h : (lambda υ).length ≤ n) :
+lemma lambda_eq_of_le' {μ : Tree 0} {υ : branch μ → option (Tree 1)} {n : ℕ} (h : (lambda υ).length ≤ n) :
   lambda' υ n = lambda υ :=
 begin
   have C : μ.length ≤ n ∨ n ≤ μ.length, from le_total _ _,
@@ -367,7 +351,7 @@ begin
     exact list.suffix_antisymm lmm₂ lmm₁ }
 end
 
-lemma lambda_initial_eq {μ : Tree α 0} (υ : branch μ → option (Tree α 1)) {n : ℕ} :
+lemma lambda_initial_eq {μ : Tree 0} (υ : branch μ → option (Tree 1)) {n : ℕ} :
   (lambda υ)↾*n = lambda' υ n :=
 begin
   have C : (lambda υ).length ≤ n ∨ n < (lambda υ).length, from le_or_lt _ _,
@@ -380,27 +364,27 @@ begin
     simp[this.1] }
 end
 
-lemma up_ne_lambda {μ : Tree α 0} (υ : branch μ → option (Tree α 1)) (μ₀ : branch μ) :
+lemma up_ne_lambda {μ : Tree 0} (υ : branch μ → option (Tree 1)) (μ₀ : branch μ) :
   υ μ₀ ≠ lambda υ := λ up,
 begin
   have : lambda υ ⊂ lambda' υ (μ.length + 1),
   { simp[lambda, lambda'],
     have : 0 < weight (lambda' υ μ.length) υ, from pos_weight_of υ ⟨_, up⟩,
-    simp[this], cases get_up_inv (lambda' υ μ.length) υ; simp[has_ssubset.ssubset] },
+    simp[this], cases convergent_derivative (lambda' υ μ.length) υ; simp[has_ssubset.ssubset] },
   have eqn : lambda' υ (μ.length + 1) = lambda υ, from lambda_eq_of_le _ μ.length.le_succ,
   simp[eqn, has_ssubset.ssubset] at this,
   contradiction
 end
 
-def assign {μ : Tree α 0} (υ : branch μ → option (Tree α 1)) (η : Tree α 1) : option (Tree α 1 × ℕ) :=
+def assign {μ : Tree 0} (υ : branch μ → option (Tree 1)) (η : Tree 1) : option (Tree 1 × ℕ) :=
 S.omega_ordering.Min
   ((η, 0) :: (η.branches.filter (λ μ₀, out μ₀ = ∞)).map (λ η₀ : branch η, (η₀.val, weight η₀.val υ)))
 
-def assignment {μ : Tree α 0} (υ : branch μ → option (Tree α 1)) : option (Tree α 1 × ℕ) := assign S υ (lambda υ)
+def assignment {μ : Tree 0} (υ : branch μ → option (Tree 1)) : option (Tree 1 × ℕ) := assign S υ (lambda υ)
 
-def up {μ : Tree α 0} (υ : branch μ → option (Tree α 1)) : option (Tree α 1) := (assignment S υ).map prod.fst
+def up {μ : Tree 0} (υ : branch μ → option (Tree 1)) : option (Tree 1) := (assignment S υ).map prod.fst
 
-lemma converge_of_up {μ : Tree α 0} (υ : branch μ → option (Tree α 1)) {η : Tree α 1} 
+lemma converge_of_up {μ : Tree 0} (υ : branch μ → option (Tree 1)) {η : Tree 1} 
   (up_μ : up S υ = some η) {μ₀ : branch μ} (up_μ₀ : υ μ₀ = η) : out μ₀ ≠ ∞ := λ div,
 begin
   simp[up, assignment, assign, option.map_eq_some'] at up_μ,
@@ -414,13 +398,13 @@ end
 
 end approx
 
-def up' (S : strategy α) : Π (η : Tree α 0) (μ : branch η), option (Tree α 1)
+def up' (S : strategy α) : Π (η : Tree 0) (μ : branch η), option (Tree 1)
 | []       ⟨μ, μ_p⟩ := by exfalso; simp* at*
 | (_ :: η) ⟨μ, _⟩   := if h : μ ⊂ᵢ η then up' η ⟨μ, h⟩ else approx.up S (up' η)
 
-def up (η : Tree α 0) : option (Tree α 1) := approx.up S (up' S η)
+def up (η : Tree 0) : option (Tree 1) := approx.up S (up' S η)
 
-@[simp] lemma up'_up_consistent {η : Tree α 0} : ∀ (μ : branch η), S.up' η μ = S.up μ.val :=
+@[simp] lemma up'_up_consistent {η : Tree 0} : ∀ (μ : branch η), S.up' η μ = S.up μ.val :=
 begin
   induction η with ν η IH,
   { intros μ, have := μ.property, simp* at* },
@@ -430,44 +414,44 @@ begin
     { refl }, { exact IH _ } }
 end
 
-def lambda' (η : Tree α 0) : ℕ → Tree α 1 := approx.lambda' (S.up' η)
+def lambda' (η : Tree 0) : ℕ → Tree 1 := approx.lambda' (S.up' η)
 
-def weight (η : Tree α 1) (μ : Tree α 0) : ℕ := approx.weight η (S.up' μ)
+def weight (η : Tree 1) (μ : Tree 0) : ℕ := approx.weight η (S.up' μ)
 
-lemma le_weight_of_suffix (η : Tree α 1) {μ₁ μ₂ : Tree α 0} (ss : μ₁ <:+ μ₂) :
+lemma le_weight_of_suffix (η : Tree 1) {μ₁ μ₂ : Tree 0} (ss : μ₁ <:+ μ₂) :
   S.weight η μ₁ ≤ S.weight η μ₂ :=
 approx.le_weight_of_suffix η ss (S.up' μ₁) (S.up' μ₂) (λ x, by simp)
 
-def lambda (η : Tree α 0) : Tree α 1 := approx.lambda (S.up' η)
+def lambda (η : Tree 0) : Tree 1 := approx.lambda (S.up' η)
 
-lemma lambda'_suffix_eq {μ : Tree α 0} {n : ℕ} {x} {η : Tree α 1} (hη : x :: η <:+ S.lambda' μ n) :
+lemma lambda'_suffix_eq {μ : Tree 0} {n : ℕ} {x} {η : Tree 1} (hη : x :: η <:+ S.lambda' μ n) :
   S.lambda' μ η.length = η ∧ S.lambda' μ (η.length + 1) = x :: η :=
-@approx.lambda'_suffix_eq _ _ μ (S.up' μ) n x η hη 
+@approx.lambda'_suffix_eq μ (S.up' μ) n x η hη 
 
-lemma converge_of_up_lt {μ : Tree α 0} {η : Tree α 1} {μ₁ μ₂ : branch μ} (lt : μ₁ < μ₂)
+lemma converge_of_up_lt {μ : Tree 0} {η : Tree 1} {μ₁ μ₂ : branch μ} (lt : μ₁ < μ₂)
   (up₁ : S.up μ₁ = η) (up₂ : S.up μ₂ = η) : out μ₁ ≠ ∞ :=
 by { have out_eqn : out μ₁ = out ⟨↑μ₁, lt⟩, from suffix_out_eq (by simp) (list.suffix_of_is_initial μ₂.property),
-     have := @approx.converge_of_up _ _ S μ₂ (S.up' μ₂) _ up₂ ⟨μ₁, lt⟩, simp[←out_eqn] at this,
+     have := @approx.converge_of_up _ S μ₂ (S.up' μ₂) _ up₂ ⟨μ₁, lt⟩, simp[←out_eqn] at this,
      exact this up₁ }
 
-lemma converge_of_up {μ : Tree α 0} {η : Tree α 1} 
+lemma converge_of_up {μ : Tree 0} {η : Tree 1} 
   (up_μ : S.up μ = η) {μ₀ : branch μ} (up_μ₀ : S.up μ₀ = η) : out μ₀ ≠ ∞ :=
-by { have := @approx.converge_of_up _ _ S μ (S.up' μ) η up_μ μ₀, simp at this, exact this up_μ₀ }
+by { have := @approx.converge_of_up _ S μ (S.up' μ) η up_μ μ₀, simp at this, exact this up_μ₀ }
 
-lemma lambda'_convergent_out_iff {μ : Tree α 0} {n : ℕ} {η : branch (S.lambda' μ n)} {μ₀ : branch μ} :
+lemma lambda'_convergent_out_iff {μ : Tree 0} {n : ℕ} {η : branch (S.lambda' μ n)} {μ₀ : branch μ} :
   out η = sum.inr μ₀.val ↔ (out μ₀ = ∞) ∧ (S.up μ₀ = η) ∧ (∀ μ₁, μ₁ < μ₀ → S.up μ₁ = η → out μ₁ ≠ ∞) :=
-by { have := @approx.lambda'_convergent_out_iff _ _ μ (S.up' μ) n η μ₀, simp at this, 
+by { have := @approx.lambda'_convergent_out_iff μ (S.up' μ) n η μ₀, simp at this, 
      exact this }
 
-lemma lambda'_convergent_out_iff' {μ : Tree α 0} {n : ℕ} {η : branch (S.lambda' μ n)} {μ₀ : Tree α 0} :
+lemma lambda'_convergent_out_iff' {μ : Tree 0} {n : ℕ} {η : branch (S.lambda' μ n)} {μ₀ : Tree 0} :
   out η = sum.inr μ₀ ↔ S.up μ₀ = η ∧ ∃ h : μ₀ ⊂ μ, (out ⟨μ₀, h⟩ = ∞) :=
 begin
-  have := @approx.lambda'_convergent_out_iff _ _ μ (S.up' μ) n η,
+  have := @approx.lambda'_convergent_out_iff μ (S.up' μ) n η,
   split,
-  { intros h, have lt : μ₀ ⊂ μ, from @approx.branch_of_out_inr _ _ μ (S.up' μ) n η μ₀ h,
-    have := (@approx.lambda'_convergent_out_iff _ _ μ (S.up' μ) n η ⟨μ₀, lt⟩).mp h,
+  { intros h, have lt : μ₀ ⊂ μ, from @approx.branch_of_out_inr μ (S.up' μ) n η μ₀ h,
+    have := (@approx.lambda'_convergent_out_iff μ (S.up' μ) n η ⟨μ₀, lt⟩).mp h,
     simp[branch.lt_iff] at this, exact ⟨this.2.1, lt, this.1⟩ },
-  { rintros ⟨up₀, lt, div⟩, have := (@approx.lambda'_convergent_out_iff _ _ μ (S.up' μ) n η ⟨μ₀, lt⟩).mpr,
+  { rintros ⟨up₀, lt, div⟩, have := (@approx.lambda'_convergent_out_iff μ (S.up' μ) n η ⟨μ₀, lt⟩).mpr,
     simp only [branch.lt_iff, up'_up_consistent] at this,
     refine this ⟨div, up₀, λ μ₁ lt₀ up₁, _⟩,
     have : out μ₁ = out ⟨↑μ₁, lt₀⟩, from suffix_out_eq (by simp) (list.suffix_of_is_initial lt), simp[this],
@@ -475,19 +459,19 @@ begin
 end
 
 lemma lambda'_divergent_out_iff
-  {μ : Tree α 0} {n : ℕ} {η : branch (S.lambda' μ n)} :
+  {μ : Tree 0} {n : ℕ} {η : branch (S.lambda' μ n)} :
   out η = ∞ ↔ (∀ μ₀ : branch μ, S.up μ₀ = η → out μ₀ ≠ ∞) :=
-by { have := @approx.lambda'_divergent_out_iff _ _ μ (S.up' μ) n η, simp at this, 
+by { have := @approx.lambda'_divergent_out_iff μ (S.up' μ) n η, simp at this, 
      exact this }
 
-lemma lambda_initial_eq {μ : Tree α 0} {n : ℕ} : (S.lambda μ)↾*n = S.lambda' μ n :=
-@approx.lambda_initial_eq _ _ μ (S.up' μ) n
+lemma lambda_initial_eq {μ : Tree 0} {n : ℕ} : (S.lambda μ)↾*n = S.lambda' μ n :=
+@approx.lambda_initial_eq μ (S.up' μ) n
 
-def assignment (μ : Tree α 0) : option (Tree α 1 × ℕ) := approx.assignment S (up' S μ)
+def assignment (μ : Tree 0) : option (Tree 1 × ℕ) := approx.assignment S (up' S μ)
 
-variables (Λ : Path α 0)
+variables (Λ : Path 0)
 
-lemma pos_of_some_ss {μ₁ μ₂ : Tree α 0} {n : ℕ} {x}
+lemma pos_of_some_ss {μ₁ μ₂ : Tree 0} {n : ℕ} {x}
   (ss : μ₁ ⊆ μ₂) (h : (S.lambda μ₁)↾*n = (S.lambda μ₂)↾*n) (d : (S.lambda μ₁).rnth n = some x) :
   0 < S.weight (S.lambda' μ₂ n) μ₂ :=
 begin
@@ -505,14 +489,14 @@ begin
     simp[lambda_initial_eq] at this, contradiction }
 end
 
-lemma some_of_some_ss (μ₁ μ₂ : Tree α 0) {n : ℕ} {x}
+lemma some_of_some_ss (μ₁ μ₂ : Tree 0) {n : ℕ} {x}
   (ss : μ₁ ⊆ μ₂) (h : (S.lambda μ₁)↾*n = (S.lambda μ₂)↾*n) (d : (S.lambda μ₁).rnth n = some x) :
   ((S.lambda μ₂).rnth n).is_some :=
 begin
   have : S.lambda' μ₂ n ⊂ᵢ S.lambda' μ₂ (n + 1),
   { have : 0 < approx.weight (approx.lambda' (S.up' μ₂) n) (S.up' μ₂), from S.pos_of_some_ss ss h d,
     simp[lambda', approx.lambda', this],
-    cases C₁ : approx.get_up_inv (approx.lambda' (S.up' μ₂) n) (S.up' μ₂); simp[C₁] },
+    cases C₁ : approx.convergent_derivative (approx.lambda' (S.up' μ₂) n) (S.up' μ₂); simp[C₁] },
   have : out ⟨S.lambda μ₂↾*n, _⟩ :: S.lambda μ₂↾*n <:+ S.lambda μ₂↾*(n + 1),
   { have := suffix_out_cons ⟨S.lambda' μ₂ n, this⟩, simp[←lambda_initial_eq] at this, exact this },
   have : list.rnth (S.lambda μ₂) n = some (out ⟨S.lambda μ₂↾*n, _⟩),
@@ -520,7 +504,7 @@ begin
   simp[this]
 end
 
-lemma inr_of_inr_ss (μ₁ μ₂ : Tree α 0) {n : ℕ} {ν : Tree α 0}
+lemma inr_of_inr_ss (μ₁ μ₂ : Tree 0) {n : ℕ} {ν : Tree 0}
   (ss : μ₁ ⊆ μ₂) (h : (S.lambda μ₁)↾*n = (S.lambda μ₂)↾*n) (d : (S.lambda μ₁).rnth n = some (sum.inr ν)) :
   (S.lambda μ₂).rnth n = some (sum.inr ν) :=
 begin
@@ -528,22 +512,22 @@ begin
   have len : (S.lambda μ₁↾*n).length = n, from list.initial_length (list.rnth_some_lt d),
   have h' : S.lambda' μ₁ n = S.lambda' μ₂ n, { simp[S.lambda_initial_eq] at h, exact h },
   have pos : 0 < approx.weight (approx.lambda' (S.up' μ₂) n) (S.up' μ₂), from S.pos_of_some_ss ss h d,
-  have : ∃ h, approx.get_up_inv (S.lambda' μ₂ n) (S.up' μ₂) = some ⟨ν, h⟩,
+  have : ∃ h, approx.convergent_derivative (S.lambda' μ₂ n) (S.up' μ₂) = some ⟨ν, h⟩,
   { have : S.lambda' μ₁ ((S.lambda μ₁↾*n).length + 1) = sum.inr ν :: S.lambda μ₁↾*n,
       from (S.lambda'_suffix_eq lmm₁).2,
     simp[len, lambda', approx.lambda'] at this,
     by_cases C₁ : 0 < approx.weight (approx.lambda' (S.up' μ₁) n) (S.up' μ₁); simp[C₁] at this,
-    { cases C₂ : approx.get_up_inv (approx.lambda' (S.up' μ₁) n) (S.up' μ₁) with ν₂; simp[C₂] at this,
+    { cases C₂ : approx.convergent_derivative (approx.lambda' (S.up' μ₁) n) (S.up' μ₁) with ν₂; simp[C₂] at this,
       { exfalso, have := list.head_eq_of_cons_eq this, simp at this, contradiction },
       { have : ↑ν₂ = ν, from sum.inr.inj_iff.mp (list.head_eq_of_cons_eq this), simp[←this],
         have : ν₂.val ⊂ᵢ μ₂, from list.suffix_of_is_initial_is_initial ν₂.property ss,
         refine ⟨this, _⟩, 
-        have C₂ : approx.get_up_inv (S.lambda' μ₂ n) (S.up' μ₁) = some ν₂, rw ←h', from C₂,
-        exact approx.get_up_inv_of_suffx (S.lambda' μ₂ n) ss (S.up' μ₁) (S.up' μ₂)
+        have C₂ : approx.convergent_derivative (S.lambda' μ₂ n) (S.up' μ₁) = some ν₂, rw ←h', from C₂,
+        exact approx.convergent_derivative_of_suffx (S.lambda' μ₂ n) ss (S.up' μ₁) (S.up' μ₂)
           (λ x, by simp) C₂} },
     { exfalso, simp[lambda_initial_eq, lambda'] at this, contradiction } },
   rcases this with ⟨i, eqn⟩,
-  have eqn' : approx.get_up_inv (approx.lambda' (S.up' μ₂) n) (S.up' μ₂) = some ⟨ν, i⟩, from eqn,
+  have eqn' : approx.convergent_derivative (approx.lambda' (S.up' μ₂) n) (S.up' μ₂) = some ⟨ν, i⟩, from eqn,
   cases C : (S.lambda μ₂).rnth n with ν₀,
   { exfalso, have := S.some_of_some_ss _ _ ss h d, simp[C] at this, contradiction },
   have : sum.inr ν :: S.lambda μ₂↾*n <:+ S.lambda μ₂↾*(n + 1),
@@ -582,7 +566,7 @@ begin
     rcases C₁ with ⟨s₁, eqn_s₁, ν, C₁⟩,
     by_cases C₂ : ∀ s, s₁ ≤ s → (S.lambda (Λ.path s)).rnth n = some ∞,
     { refine ⟨s₁, eqn_s₁, λ s eqn_s, _⟩, simp[C₂, C₂ s eqn_s] },
-    have C₂ : ∃ s₂, s₁ ≤ s₂ ∧ ∃ (ν : Tree α 0), (S.lambda (Λ.path s₂)).rnth n = some (sum.inr ν),
+    have C₂ : ∃ s₂, s₁ ≤ s₂ ∧ ∃ (ν : Tree 0), (S.lambda (Λ.path s₂)).rnth n = some (sum.inr ν),
     { simp at C₂, rcases C₂ with ⟨s₂, eqn_s₂, C₂⟩,
       refine ⟨s₂, eqn_s₂, _⟩,
       have : ((S.lambda (Λ.path s₂)).rnth n).is_some,
@@ -603,7 +587,7 @@ begin
 end 
 
 theorem finite_injury' :
-  ∃ Λ' : Path α 1, ∀ n, ∃ s₀, ∀ s, s₀ ≤ s → S.lambda (Λ.path s)↾*n = Λ'.path n :=
+  ∃ Λ' : Path 1, ∀ n, ∃ s₀, ∀ s, s₀ ≤ s → S.lambda (Λ.path s)↾*n = Λ'.path n :=
 begin
   let P : ℕ → ℕ → Prop := λ n s₀, (∀ s, s₀ ≤ s → S.lambda (Λ.path s)↾*n = S.lambda (Λ.path s₀)↾*n),
   have : ∀ n, ∃ s₀, P n s₀, from λ n, S.finite_injury Λ n,
@@ -612,7 +596,7 @@ begin
   have : ∃ (f : ℕ → ℕ), ∀ x, (∀ s, s < f x → ¬P x s) ∧ P x (f x),
     from classical.skolem.mp this,
   rcases this with ⟨f, h_f⟩,
-  let path : ℕ → Tree α 1 := λ n, S.lambda (Λ.path (f n))↾*n,
+  let path : ℕ → Tree 1 := λ n, S.lambda (Λ.path (f n))↾*n,
   have mono : ∀ n, path n <:+ path (n + 1),
   { intros n, simp[path],
     have mono : f n ≤ f (n + 1),
@@ -632,13 +616,13 @@ begin
   exact (h_f n).2 _ eqn_s
 end
 
-noncomputable def Lambda (Λ : Path α 0) : Path α 1 := classical.epsilon
+noncomputable def Lambda (Λ : Path 0) : Path 1 := classical.epsilon
 (λ Λ',  ∀ n, ∃ s₀, ∀ s, s₀ ≤ s → S.lambda (Λ.path s)↾*n = Λ'.path n)
 
 theorem Lambda_spec : ∀ n, ∃ s₀, ∀ s, s₀ ≤ s → S.lambda (Λ.path s)↾*n = (S.Lambda Λ).path n :=
 classical.epsilon_spec (S.finite_injury' Λ)
 
-theorem Lambda_converge {n} {η : branch ((S.Lambda Λ).path n)} {μ : Tree α 0} :
+theorem Lambda_converge {n} {η : branch ((S.Lambda Λ).path n)} {μ : Tree 0} :
   out η = sum.inr μ ↔ S.up μ = η ∧ ∃ {n} (h : μ ⊂ Λ.path n), out ⟨μ, h⟩ = ∞ :=
 begin
     have := S.Lambda_spec Λ n, rcases this with ⟨s₀, h⟩,
@@ -650,7 +634,7 @@ begin
     out η = sum.inr μ ↔ S.up μ = ↑η ∧ ∃ (h : μ ⊂ (Λ.path s)), out ⟨μ, h⟩ = ∞,
   { intros s eqn,
     have out_eq : out ⟨η.val, (ini eqn)⟩ = out η, from suffix_out_eq (by simp) (suf eqn),
-    have := @lambda'_convergent_out_iff' _ _ S (Λ.path s) _ ⟨η.val, (ini eqn)⟩ μ,
+    have := @lambda'_convergent_out_iff' _ S (Λ.path s) _ ⟨η.val, (ini eqn)⟩ μ,
     rw out_eq at this, exact this },
   split,
   { intros h, have := (out_iff s₀ (by simp)).mp h, refine ⟨this.1, s₀, this.2⟩ },
@@ -672,7 +656,7 @@ begin
     out η = ∞ ↔ ∀ (μ₀ : branch (Λ.path s)), S.up ↑μ₀ = ↑η.val → out μ₀ ≠ ∞,
   { intros s eqn,
     have out_eq : out ⟨η.val, (ini eqn)⟩ = out η, from suffix_out_eq (by simp) (suf eqn),
-    have := @lambda'_divergent_out_iff _ _ S (Λ.path s) _ ⟨η.val, (ini eqn)⟩,
+    have := @lambda'_divergent_out_iff _ S (Λ.path s) _ ⟨η.val, (ini eqn)⟩,
     rw out_eq at this, exact this },
   split,
   { intros h s μ,
@@ -683,11 +667,13 @@ begin
   { intros h, simp[out_iff s₀ (by simp)], exact @h s₀ }
 end
 
-@[simp] def computation_path_aux : ℕ → Tree α 0
-| 0       := []
-| (s + 1) := S.computation (computation_path_aux s) (S.assignment (computation_path_aux s)) :: computation_path_aux s
+@[simp] def computation_path_aux : ℕ → Tree 0 × α
+| 0       := ([], S.computation_init)
+| (s + 1) := let μ := (computation_path_aux s).1, state := (computation_path_aux s).2 in
+    ((S.computation (S.assignment μ) state).1 :: μ, (S.computation (S.assignment μ) state).2)
+  
 
-def computation_path : Path α 0 := ⟨S.computation_path_aux, by simp⟩
+def computation_path : Path 0 := ⟨λ n, (S.computation_path_aux n).1, by simp⟩
 
 end strategy
 
